src/SelectBeh.v
@@ -1,6 +1,7 @@
 From sflib Require Import sflib.
 From ITree Require Export ITree.
 From Paco Require Import paco.
+(* From Ordinal Require Import Ordinal. *)
 
 Export ITreeNotations.
 
@@ -12,16 +13,17 @@ From Fairness Require Import FairBeh.
 
 Set Implicit Arguments.
 
-Section FAIR.
+Section RAWEVENT.
   Context {Ident: ID}.
 
-  Variant fairE: Type :=
-    | fairE_fair (m: id -> Flag.t)
+  Variant silentE: Type :=
+    | silentE_tau
+    | silentE_fair (m: id -> Flag.t)
   .
 
-  Definition fairO := (fairE + obsE)%type.
+  Definition rawE := (silentE + obsE)%type.
 
-End FAIR.
+End RAWEVENT.
 
 Module RawTr.
 Section TR.
@@ -29,13 +31,13 @@ Section TR.
 
   CoInductive t {R}: Type :=
   | done (retv: R)
-  | spin
+  (* | spin *)
   | ub
   | nb
-  | cons (hd: fairO) (tl: t)
+  | cons (hd: rawE) (tl: t)
   .
 
-  Fixpoint app {R} (pre: list fairO) (bh: @t R): t :=
+  Fixpoint app {R} (pre: list rawE) (bh: @t R): t :=
     match pre with
     | [] => bh
     | hd :: tl => cons hd (app tl bh)
@@ -49,124 +51,192 @@ Section TR.
   .
   Proof. reflexivity. Qed.
 
-  Definition prefix {R} (pre: list fairO) (bh: @t R): Prop :=
+  Definition prefix {R} (pre: list rawE) (bh: @t R): Prop :=
     exists tl, <<PRE: app pre tl = bh>>
   .
 
-  Variant _nofail_id
-          (nofail_id: forall (R: Type) (i: id), (@t R) -> Prop)
+
+  (** select fair trace with induction **)
+  Variant _nofail_ind
+          (nofail_ind: forall (R: Type) (i: id), (@t R) -> Prop)
           (R: Type) (i: id)
     :
     (@t R) -> Prop :=
-    | nofail_id_done
+    | nofail_ind_done
         retv
       :
-      _nofail_id nofail_id i (done retv)
-    | nofail_id_spin
+      _nofail_ind nofail_ind i (done retv)
+    (* | nofail_ind_spin *)
+    (*   : *)
+    (*   _nofail_ind nofail_ind i spin *)
+    | nofail_ind_ub
       :
-      _nofail_id nofail_id i spin
-    | nofail_id_ub
+      _nofail_ind nofail_ind i ub
+    | nofail_ind_nb
       :
-      _nofail_id nofail_id i ub
-    | nofail_id_nb
-      :
-      _nofail_id nofail_id i nb
-    | nofail_id_obs
+      _nofail_ind nofail_ind i nb
+    | nofail_ind_obs
         (obs: obsE) tl
-        (TL: nofail_id R i tl)
+        (TL: nofail_ind R i tl)
       :
-      _nofail_id nofail_id i (cons (inr obs) tl)
-    | nofail_id_fair
+      _nofail_ind nofail_ind i (cons (inr obs) tl)
+    | nofail_ind_fair
         fmap tl
         (NOFAIL: Flag.le Flag.emp (fmap i))
-        (TL: nofail_id R i tl)
+        (TL: nofail_ind R i tl)
       :
-      _nofail_id nofail_id i (cons (inl (fairE_fair fmap)) tl)
+      _nofail_ind nofail_ind i (cons (inl (silentE_fair fmap)) tl)
+    | nofail_ind_tau
+        tl
+        (TL: nofail_ind R i tl)
+      :
+      _nofail_ind nofail_ind i (cons (inl silentE_tau) tl)
   .
 
-  Definition nofail_id: forall (R: Type) (i: id), (@t R) -> Prop := paco3 _nofail_id bot3.
+  Definition nofail_ind: forall (R: Type) (i: id), (@t R) -> Prop := paco3 _nofail_ind bot3.
 
-  Lemma nofail_id_mon: monotone3 _nofail_id.
+  Lemma nofail_ind_mon: monotone3 _nofail_ind.
   Proof.
     ii. inv IN; econs; eauto.
   Qed.
 
 
-  Inductive _fair_id
-            (fair_id: forall (R: Type) (i: id), (@t R) -> Prop)
+  Inductive _fair_ind
+            (fair_ind: forall (R: Type) (i: id), (@t R) -> Prop)
             (R: Type) (i: id)
     :
     (@t R) -> Prop :=
-  | fair_id_nofail
+  | fair_ind_nofail
       tr
-      (NOFAIL: nofail_id i tr)
+      (NOFAIL: nofail_ind i tr)
     :
-    _fair_id fair_id i tr
-  | fair_id_no_success
+    _fair_ind fair_ind i tr
+  | fair_ind_no_success
       fmap tl
       (NOSUCCESS: Flag.le (fmap i) Flag.emp)
-      (TL: _fair_id fair_id i tl)
+      (TL: _fair_ind fair_ind i tl)
     :
-    _fair_id fair_id i (cons (inl (fairE_fair fmap)) tl)
-  | fair_id_obs
+    _fair_ind fair_ind i (cons (inl (silentE_fair fmap)) tl)
+  | fair_ind_tau
+      tl
+      (TL: _fair_ind fair_ind i tl)
+    :
+    _fair_ind fair_ind i (cons (inl silentE_tau) tl)
+  | fair_ind_obs
       (obs: obsE) tl
-      (TL: _fair_id fair_id i tl)
+      (TL: _fair_ind fair_ind i tl)
     :
-    _fair_id fair_id i (cons (inr obs) tl)
-  | fair_id_success
+    _fair_ind fair_ind i (cons (inr obs) tl)
+  | fair_ind_success
       fmap tl
       (SUCCESS: Flag.le Flag.success (fmap i))
-      (TL: fair_id R i tl)
+      (TL: fair_ind R i tl)
     :
-    _fair_id fair_id i (cons (inl (fairE_fair fmap)) tl)
+    _fair_ind fair_ind i (cons (inl (silentE_fair fmap)) tl)
   .
 
-  Definition fair_id: forall (R: Type) (i: id), (@t R) -> Prop := paco3 _fair_id bot3.
+  Definition fair_ind: forall (R: Type) (i: id), (@t R) -> Prop := paco3 _fair_ind bot3.
 
-  Lemma fair_id_ind
+  Lemma fair_ind_ind
         (r: forall (R: Type) (i: id), t -> Prop) R i (P: t -> Prop)
-        (NOFAIL: forall tr (NOFAIL: nofail_id i tr), P tr)
+        (NOFAIL: forall tr (NOFAIL: nofail_ind i tr), P tr)
         (NOSUCCESS: forall fmap tl
                       (NOSUCCESS: Flag.le (fmap i) Flag.emp)
-                      (FAIRID: _fair_id r i tl)
+                      (TL: _fair_ind r i tl)
                       (IH: P tl),
-            P (cons (inl (fairE_fair fmap)) tl))
+            P (cons (inl (silentE_fair fmap)) tl))
+        (TAU: forall tl
+                (TL: _fair_ind r i tl)
+                (IH: P tl),
+            P (cons (inl silentE_tau) tl))
         (OBS: forall obs tl
-                (FAIRID: _fair_id r i tl)
+                (TL: _fair_ind r i tl)
                 (IH: P tl),
             P (cons (inr obs) tl))
         (SUCCESS: forall fmap tl
                     (SUCCESS: Flag.le Flag.success (fmap i))
-                    (FAIRID: r R i tl),
-            P (cons (inl (fairE_fair fmap)) tl))
+                    (TL: r R i tl),
+            P (cons (inl (silentE_fair fmap)) tl))
     :
-    forall tr, _fair_id r i tr -> P tr.
+    forall tr, _fair_ind r i tr -> P tr.
   Proof.
     fix IH 2. i.
     inv H; eauto.
   Qed.
 
-  Lemma fair_id_mon: monotone3 _fair_id.
+  Lemma fair_ind_mon: monotone3 _fair_ind.
   Proof.
-    ii. induction IN using fair_id_ind; eauto.
+    ii. induction IN using fair_ind_ind; eauto.
     - econs 1. eauto.
     - econs 2; eauto.
     - econs 3; eauto.
     - econs 4; eauto.
+    - econs 5; eauto.
   Qed.
 
-  Definition is_fair {R} (tr: @t R) := forall i, fair_id i tr.
+  Definition is_fair_ind {R} (tr: @t R) := forall i, fair_ind i tr.
+
+
+  (** select fair trace with well-founded order **)
+  (* Context {WFOrd: WFO}. *)
+
+  Variant _fair_ord
+          (fair_ord: forall (R: Type) (m: imap), (@t R) -> Prop)
+          (R: Type) (m: imap)
+    :
+    (@t R) -> Prop :=
+    | fair_ord_done
+        retv
+      :
+      _fair_ord fair_ord m (done retv)
+    (* | nofail_ind_spin *)
+    (*   : *)
+    (*   _nofail_ind nofail_ind i spin *)
+    | fair_ord_ub
+      :
+      _fair_ord fair_ord m ub
+    | fair_ord_nb
+      :
+      _fair_ord fair_ord m nb
+    | fair_ord_obs
+        (obs: obsE) tl
+        (TL: fair_ord R m tl)
+      :
+      _fair_ord fair_ord m (cons (inr obs) tl)
+    | fair_ord_fair
+        fmap tl m0
+        (FAIR: fair_update m m0 fmap)
+        (TL: fair_ord R m0 tl)
+      :
+      _fair_ord fair_ord m (cons (inl (silentE_fair fmap)) tl)
+    | fair_ord_tau
+        tl
+        (TL: fair_ord R m tl)
+      :
+      _fair_ord fair_ord m (cons (inl silentE_tau) tl)
+  .
+
+  Definition fair_ord: forall (R: Type) (m: imap), (@t R) -> Prop := paco3 _fair_ord bot3.
+
+  Lemma fair_ord_mon: monotone3 _fair_ord.
+  Proof.
+    ii. inv IN; econs; eauto.
+  Qed.
+
+  Definition is_fair_ord {R} (tr: @t R) := exists m, fair_ord m tr.
 
 End TR.
 End RawTr.
-#[export] Hint Constructors RawTr._nofail_id.
-#[export] Hint Unfold RawTr.nofail_id.
-#[export] Hint Resolve RawTr.nofail_id_mon: paco.
+#[export] Hint Constructors RawTr._nofail_ind.
+#[export] Hint Unfold RawTr.nofail_ind.
+#[export] Hint Resolve RawTr.nofail_ind_mon: paco.
+#[export] Hint Constructors RawTr._fair_ind.
+#[export] Hint Unfold RawTr.fair_ind.
+#[export] Hint Resolve RawTr.fair_ind_mon: paco.
+#[export] Hint Constructors RawTr._fair_ord.
+#[export] Hint Unfold RawTr.fair_ord.
+#[export] Hint Resolve RawTr.fair_ord_mon: paco.
 #[export] Hint Resolve cpn3_wcompat: paco.
-#[export] Hint Constructors RawTr._fair_id.
-#[export] Hint Unfold RawTr.fair_id.
-#[export] Hint Resolve RawTr.fair_id_mon: paco.
-
 
 
 Module RawBeh.
@@ -177,45 +247,45 @@ Section BEHAVES.
   Definition t {R}: Type := @RawTr.t _ R -> Prop.
   Definition improves {R} (src tgt: @t R): Prop := tgt <1= src.
 
-  Variant _diverge
-          (diverge: forall (R: Type) (itr: @state _ R), Prop)
-          (R: Type)
-    :
-    forall (itr: @state _ R), Prop :=
-    | diverge_tau
-        itr
-        (DIV: diverge _ itr)
-      :
-      _diverge diverge (Tau itr)
-    | diverge_choose
-        X ktr x
-        (DIV: diverge _ (ktr x))
-      :
-      _diverge diverge (Vis (Choose X) ktr)
-    | diverge_ub
-        ktr
-      :
-      _diverge diverge (Vis Undefined ktr)
-  .
+  (* Variant _diverge *)
+  (*         (diverge: forall (R: Type) (itr: @state _ R), Prop) *)
+  (*         (R: Type) *)
+  (*   : *)
+  (*   forall (itr: @state _ R), Prop := *)
+  (*   | diverge_tau *)
+  (*       itr *)
+  (*       (DIV: diverge _ itr) *)
+  (*     : *)
+  (*     _diverge diverge (Tau itr) *)
+  (*   | diverge_choose *)
+  (*       X ktr x *)
+  (*       (DIV: diverge _ (ktr x)) *)
+  (*     : *)
+  (*     _diverge diverge (Vis (Choose X) ktr) *)
+  (*   | diverge_ub *)
+  (*       ktr *)
+  (*     : *)
+  (*     _diverge diverge (Vis Undefined ktr) *)
+  (* . *)
 
-  Lemma diverge_mon: monotone2 _diverge.
-  Proof.
-    ii. inv IN.
-    - econs 1; eauto.
-    - econs 2; eauto.
-    - econs 3; eauto.
-  Qed.
+  (* Lemma diverge_mon: monotone2 _diverge. *)
+  (* Proof. *)
+  (*   ii. inv IN. *)
+  (*   - econs 1; eauto. *)
+  (*   - econs 2; eauto. *)
+  (*   - econs 3; eauto. *)
+  (* Qed. *)
 
-  Definition diverge: forall (R: Type) (itr: state), Prop := paco2 _diverge bot2.
+  (* Definition diverge: forall (R: Type) (itr: state), Prop := paco2 _diverge bot2. *)
 
-  Hint Constructors _diverge.
-  Hint Unfold diverge.
-  Hint Resolve diverge_mon: paco.
-  Hint Resolve cpn2_wcompat: paco.
+  (* Hint Constructors _diverge. *)
+  (* Hint Unfold diverge. *)
+  (* Hint Resolve diverge_mon: paco. *)
+  (* Hint Resolve cpn2_wcompat: paco. *)
 
 
 
-  Inductive _of_state
+  Variant _of_state
             (of_state: forall (R: Type), (@state _ R) -> (@RawTr.t _ R) -> Prop)
             (R: Type)
     :
@@ -224,11 +294,11 @@ Section BEHAVES.
       retv
     :
     _of_state of_state (Ret retv) (RawTr.done retv)
-  | spin
-      st0
-      (SPIN: diverge st0)
-    :
-    _of_state of_state st0 (RawTr.spin)
+  (* | spin *)
+  (*     st0 *)
+  (*     (SPIN: diverge st0) *)
+  (*   : *)
+  (*   _of_state of_state st0 (RawTr.spin) *)
   | nb
       st0
     :
@@ -240,21 +310,20 @@ Section BEHAVES.
     _of_state of_state (Vis (Observe fn args) ktr) (RawTr.cons (inr (obsE_syscall fn args rv)) tl)
 
   | tau
-      itr tr
-      (STEP: _of_state of_state itr tr)
+      itr tl
+      (TL: of_state _ itr tl)
     :
-    _of_state of_state (Tau itr) tr
+    _of_state of_state (Tau itr) (RawTr.cons (inl silentE_tau) tl)
   | choose
-      X ktr x tr
-      (STEP: _of_state of_state (ktr x) tr)
+      X ktr x tl
+      (TL: of_state _ (ktr x) tl)
     :
-    _of_state of_state (Vis (Choose X) ktr) tr
-
+    _of_state of_state (Vis (Choose X) ktr) (RawTr.cons (inl silentE_tau) tl)
   | fair
       fmap ktr tl
       (TL: of_state _ (ktr tt) tl)
     :
-    _of_state of_state (Vis (Fair fmap) ktr) (RawTr.cons (inl (fairE_fair fmap)) tl)
+    _of_state of_state (Vis (Fair fmap) ktr) (RawTr.cons (inl (silentE_fair fmap)) tl)
 
   | ub
       ktr tr
@@ -264,49 +333,9 @@ Section BEHAVES.
 
   Definition of_state: forall (R: Type), state -> RawTr.t -> Prop := paco3 _of_state bot3.
 
-  Theorem of_state_ind:
-    forall (r: forall (R: Type), state -> RawTr.t -> Prop) R (P: state -> RawTr.t -> Prop),
-      (forall retv, P (Ret retv) (RawTr.done retv)) ->
-      (forall st0, diverge st0 -> P st0 RawTr.spin) ->
-      (forall st0, P st0 RawTr.nb) ->
-      (forall fn args rv ktr tl
-         (TL: r _ (ktr rv) tl)
-        ,
-          P (Vis (Observe fn args) ktr) (RawTr.cons (inr (obsE_syscall fn args rv)) tl)) ->
-      (forall itr tr
-         (STEP: _of_state r itr tr)
-         (IH: P itr tr)
-        ,
-          P (Tau itr) tr) ->
-      (forall X ktr x tr
-         (STEP: _of_state r (ktr x) tr)
-         (IH: P (ktr x) tr)
-        ,
-          P (Vis (Choose X) ktr) tr) ->
-      (forall fmap ktr tl
-         (TL: r _ (ktr tt) tl)
-        ,
-          P (Vis (Fair fmap) ktr) (RawTr.cons (inl (fairE_fair fmap)) tl)) ->
-      (forall ktr tr, P (Vis Undefined ktr) tr) ->
-      forall s t, @_of_state r R s t -> P s t.
-  Proof.
-    fix IH 14. i.
-    inv H7; eauto.
-    - eapply H3; eauto. eapply IH; eauto.
-    - eapply H4; eauto. eapply IH; eauto.
-  Qed.
-
   Lemma of_state_mon: monotone3 _of_state.
   Proof.
-    ii. induction IN using of_state_ind; eauto.
-    - econs 1; eauto.
-    - econs 2; eauto.
-    - econs 3; eauto.
-    - econs 4; eauto.
-    - econs 5; eauto.
-    - econs 6; eauto.
-    - econs 7; eauto.
-    - econs 8; eauto.
+    ii. inv IN; econs; eauto.
   Qed.
 
   Hint Constructors _of_state.
@@ -314,76 +343,11 @@ Section BEHAVES.
   Hint Resolve of_state_mon: paco.
   Hint Resolve cpn3_wcompat: paco.
 
-  Definition of_state_fair {R} (st: @state _ R) (raw_tr: @RawTr.t _ R) :=
-    (<<BEH: of_state st raw_tr>>) /\ (<<FAIR: RawTr.is_fair raw_tr>>).
+  Definition of_state_fair_ind {R} (st: @state _ R) (raw_tr: @RawTr.t _ R) :=
+    (<<BEH: of_state st raw_tr>>) /\ (<<FAIR: RawTr.is_fair_ind raw_tr>>).
 
-  (****************************************************)
-  (*********************** upto ***********************)
-  (****************************************************)
-
-  Variant of_state_indC
-          (of_state: forall R, (@state _ R) -> (@RawTr.t _ R) -> Prop)
-          R
-    :
-    (@state _ R) -> (@RawTr.t _ R) -> Prop :=
-  | of_state_indC_done
-      retv
-    :
-    of_state_indC of_state (Ret retv) (RawTr.done retv)
-  | of_state_indC_spin
-      st0
-      (SPIN: diverge st0)
-    :
-    of_state_indC of_state st0 (RawTr.spin)
-  | of_state_indC_nb
-      st0
-    :
-    of_state_indC of_state st0 (RawTr.nb)
-  | of_state_indC_obs
-      fn args rv ktr tl
-      (TL: of_state _ (ktr rv) tl)
-    :
-    of_state_indC of_state (Vis (Observe fn args) ktr) (RawTr.cons (inr (obsE_syscall fn args rv)) tl)
-
-  | of_state_indC_tau
-      itr tr
-      (STEP: of_state _ itr tr)
-    :
-    of_state_indC of_state (Tau itr) tr
-  | of_state_indC_choose
-      X ktr x tr
-      (STEP: of_state _ (ktr x) tr)
-    :
-    of_state_indC of_state (Vis (Choose X) ktr) tr
-  | of_state_indC_fair
-      fmap ktr tl
-      (TL: of_state _ (ktr tt) tl)
-    :
-    of_state_indC of_state (Vis (Fair fmap) ktr) (RawTr.cons (inl (fairE_fair fmap)) tl)
-
-  | of_state_indC_ub
-      ktr tr
-    :
-    of_state_indC of_state (Vis Undefined ktr) tr
-  .
-
-  Lemma of_state_indC_mon: monotone3 of_state_indC.
-  Proof. ii. inv IN; econs; eauto. Qed.
-
-  Hint Resolve of_state_indC_mon: paco.
-
-  Lemma of_state_indC_wrespectful: wrespectful3 _of_state of_state_indC.
-  Proof.
-    econs; eauto with paco.
-    i. inv PR; eauto.
-    { econs; eauto. eapply rclo3_base. eauto. }
-    { econs; eauto. eapply of_state_mon; eauto. i. eapply rclo3_base. auto. }
-    { econs; eauto. eapply of_state_mon; eauto. i. eapply rclo3_base. auto. }
-    { econs; eauto. eapply rclo3_base. eauto. }
-  Qed.
-
-  Lemma of_state_indC_spec: of_state_indC <4= gupaco3 _of_state (cpn3 _of_state).
-  Proof. i. eapply wrespect3_uclo; eauto with paco. eapply of_state_indC_wrespectful. Qed.
+  Definition of_state_fair_ord {R} (st: @state _ R) (raw_tr: @RawTr.t _ R) :=
+    (<<BEH: of_state st raw_tr>>) /\ (<<FAIR: RawTr.is_fair_ord raw_tr>>).
 
 
 
@@ -402,13 +366,13 @@ Section BEHAVES.
     revert_until Ident. pcofix CIH. i. punfold BEH. rr in PRE. des; subst.
     destruct pre; ss; clarify.
     { pfold. econs. }
-    remember (RawTr.cons f (RawTr.app pre tl)) as tmp. revert Heqtmp.
-    induction BEH using of_state_ind; ii; ss; clarify.
+    remember (RawTr.cons r0 (RawTr.app pre tl)) as tmp. revert Heqtmp.
+    inv BEH; ii; ss; clarify.
     - pclearbot. pfold. econs; eauto. right. eapply CIH; eauto. rr; eauto.
-    - pfold. econs 5; eauto. hexploit IHBEH; eauto. intro A. punfold A.
-    - pfold. econs 6; eauto. hexploit IHBEH; eauto. intro A. punfold A.
-    - pfold. econs 7; eauto. right. eapply CIH. pclearbot. eapply TL. rr; eauto.
-    - pfold. econs 8; eauto.
+    - pclearbot. pfold. econs 4; eauto. right. eapply CIH; eauto. rr; eauto.
+    - pclearbot. pfold. econs 5; eauto. right. eapply CIH; eauto. rr; eauto.
+    - pclearbot. pfold. econs 6; eauto. right. eapply CIH; eauto. rr; eauto.
+    - pclearbot. pfold. econs 7; eauto.
   Qed.
 
   (* Theorem prefix_closed *)
@@ -437,80 +401,13 @@ Section BEHAVES.
   .
   Proof.
     pfold. i. punfold UB.
-    remember RawTr.ub as tmp. revert Heqtmp.
-    induction UB using of_state_ind; ii; ss; clarify.
-    - econs; eauto.
-    - econs 6; eauto.
-  Qed.
-
-  Lemma beh_tau
-        R itr tr
-        (BEH: @of_state R itr tr)
-    :
-    <<BEH: of_state (Tau itr) tr>>
-  .
-  Proof.
-    ginit. guclo of_state_indC_spec. econs; eauto. gfinal. eauto.
-  Qed.
-
-  Lemma beh_choose
-        R X ktr x tr
-        (BEH: @of_state R (ktr x) tr)
-    :
-    <<BEH: of_state (Vis (Choose X) ktr) tr>>
-  .
-  Proof.
-    ginit. guclo of_state_indC_spec. econs; eauto. gfinal. eauto.
+    remember RawTr.ub as tmp. inv UB; ss; clarify.
   Qed.
 
 End BEHAVES.
 End RawBeh.
 #[export] Hint Unfold RawBeh.improves.
-#[export] Hint Constructors RawBeh._diverge.
-#[export] Hint Unfold RawBeh.diverge.
-#[export] Hint Resolve RawBeh.diverge_mon: paco.
 #[export] Hint Constructors RawBeh._of_state.
 #[export] Hint Unfold RawBeh.of_state.
 #[export] Hint Resolve RawBeh.of_state_mon: paco.
-
-#[export] Hint Resolve cpn2_wcompat: paco.
 #[export] Hint Resolve cpn3_wcompat: paco.
-
-
-Section AUX.
-
-  Context {Ident: ID}.
-
-  Theorem of_state_ind2:
-    forall R (P: state -> RawTr.t -> Prop),
-      (forall retv, P (Ret retv) (RawTr.done retv)) ->
-      (forall st0, RawBeh.diverge st0 -> P st0 RawTr.spin) ->
-      (forall st0, P st0 RawTr.nb) ->
-      (forall fn args rv ktr tl
-         (TL: RawBeh.of_state (ktr rv) tl)
-        ,
-          P (Vis (Observe fn args) ktr) (RawTr.cons (inr (obsE_syscall fn args rv)) tl)) ->
-      (forall itr tr
-         (STEP: RawBeh.of_state itr tr)
-         (IH: P itr tr)
-        ,
-          P (Tau itr) tr) ->
-      (forall X ktr x tr
-         (STEP: RawBeh.of_state (ktr x) tr)
-         (IH: P (ktr x) tr)
-        ,
-          P (Vis (Choose X) ktr) tr) ->
-      (forall fmap ktr tl
-         (TL: RawBeh.of_state (ktr tt) tl)
-        ,
-          P (Vis (Fair fmap) ktr) (RawTr.cons (inl (fairE_fair fmap)) tl)) ->
-      (forall ktr tr, P (Vis Undefined ktr) tr) ->
-      forall s t, (@RawBeh.of_state _ R s t) -> P s t.
-  Proof.
-    i. eapply RawBeh.of_state_ind; eauto.
-    { i. eapply H3; eauto. pfold. eapply RawBeh.of_state_mon; eauto. }
-    { i. eapply H4; eauto. pfold. eapply RawBeh.of_state_mon; eauto. }
-    { punfold H7. eapply RawBeh.of_state_mon; eauto. i. pclearbot. eauto. }
-  Qed.
-
-End AUX.
